Fine-grained probing works on an end-to-end example FineGrainedProbe.3d

src/3d/ocaml/lexer.mll
@@ -66,7 +66,8 @@ let () =
   H.add keywords "union" UNION;
   H.add keywords "extern" EXTERN;
   H.add keywords "probe" PROBE;
-  H.add keywords "pointer" POINTER
+  H.add keywords "pointer" POINTER;
+  H.add keywords "PURE" PURE
 
 let unsigned_int_of_string s = int_of_string (String.sub s 0 (String.length s - 2))
 
