src/3d/TranslateForInterpreter.fst
@@ -594,9 +594,9 @@ let rec parse_typ (env:global_env)
   | T.T_pointer _ _ ->
     failwith "No parsers for pointer types"
 
-  | T.T_with_probe content_type integer_type probe len dest -> 
+  | T.T_with_probe content_type integer_type probe dest -> 
     let p = parse_typ env typename fieldname content_type in
-    let q = T.Parse_with_probe p probe len dest in
+    let q = T.Parse_with_probe p probe dest in
     let u64_or_u32, _ = translate_typ (A.type_of_integer_type integer_type) in
     let u64_or_u32_parser = parse_typ env typename fieldname u64_or_u32 in
     { p_kind = u64_or_u32_parser.p_kind;
@@ -756,7 +756,7 @@ let rec parser_is_constant_size_without_actions
   | T.Parse_with_action _ _ _
   | T.Parse_if_else _ _ _
   | T.Parse_string _ _
-  | T.Parse_with_probe _ _ _ _
+  | T.Parse_with_probe _ _ _
     -> false
   | T.Parse_map p _
   | T.Parse_refinement _ p _
@@ -777,22 +777,58 @@ let make_zero (r: range) (t: typ) : ML T.expr =
   let it = typ_as_integer_type t in
   (T.Constant (Int it 0), r)
 
+let rec translate_action_as_probe_action (a:A.probe_action) : ML (T.probe_action & T.decls) =
+  let translate_atomic (a:A.probe_atomic_action) : ML T.atomic_probe_action =
+    match a with
+    | A.Probe_action_return e ->
+      T.Probe_return { value = translate_expr e }
+    | A.Probe_action_call f args ->
+      T.Probe_call_pure { f; args = List.map translate_expr args }
+    | A.Probe_action_read f ->
+      T.Probe_and_read { reader=f }
+    | A.Probe_action_write f v ->
+      T.Write_at_offset { writer=f; value=translate_expr v }
+    | A.Probe_action_copy f v ->
+      T.Probe_and_copy { bytes_to_read=translate_expr v; probe_fn=f }
+  in
+  match a.v with
+  | A.Probe_atomic_action a ->
+    T.Probe_atomic (translate_atomic a), []
+  | A.Probe_action_seq hd tl ->
+    let hd = translate_atomic hd in
+    let tl, ds2 = translate_action_as_probe_action tl in
+    T.Probe_seq {hd; tl}, ds2
+  | A.Probe_action_let i a k ->
+    let a = translate_atomic a in
+    let tl, ds2 = translate_action_as_probe_action k in
+    T.Probe_let {i; a; tl}, ds2
+
 #push-options "--z3rlimit_factor 4"
 let translate_atomic_field (f:A.atomic_field) : ML (T.struct_field & T.decls) =
   let sf = f.v in
+  let translate_probe_call (p:probe_call) : ML (T.probe_action & A.ident & T.decls) =
+    match p with
+    | SimpleCall { probe_dest; probe_length; probe_fn = Some probe_fn } ->
+      let len = translate_expr probe_length in
+      let probe_action = T.Probe_fn_as_probe_m { bytes_to_read = len; probe_fn } in
+      probe_action, probe_dest, []
+    | CompositeCall { probe_dest; probe_block } ->
+      let probe_block, ds = translate_action_as_probe_action probe_block in
+      probe_block, probe_dest, ds
+    | _ ->
+      failwith "Impossible: probe function must be resolved"
+  in
   match f.v.field_probe with
-  | Some (CompositeCall _) -> failwith ""
-  | Some (SimpleCall probe_call) -> (
-    match f.v.field_type.v, probe_call.probe_fn with
-    | Pointer t (Some (PQ a)), Some probe_fn ->
+  | Some probe_call -> (
+    let probe_action, dest, ds = translate_probe_call probe_call in
+    match f.v.field_type.v with
+    | Pointer t (Some (PQ a)) ->
       let t, ds1 = translate_typ t in
-      let len = translate_expr probe_call.probe_length in
-      let dest = probe_call.probe_dest in
-      let sf_typ = T.T_with_probe t a probe_fn len dest in
+      let sf_typ = T.T_with_probe t a probe_action dest in
       T.({ sf_dependence=sf.field_dependence;
            sf_ident=sf.field_ident;
            sf_typ=sf_typ }), 
-      ds1
+      ds@ds1
       
     | _ -> 
       failwith "Impossible: probed fields must be pointers and the probe function must be resolved"
@@ -1063,7 +1099,7 @@ let rec hoist_typ
       d, T_with_comment t c
 
     | T_pointer _ _
-    | T_with_probe _ _ _ _ _ ->
+    | T_with_probe _ _ _ _ ->
       [], t
 
 let add_parser_kind_nz (genv:global_env) (id:A.ident) (nz:bool) (wk: weak_kind) =
@@ -1320,15 +1356,25 @@ let translate_decl (env:global_env) (d:A.decl) : ML (list T.decl) =
 
   | ExternType tdnames -> [with_comments (T.Extern_type tdnames.typedef_abbrev) (A.is_entrypoint d) false []]
 
-  | ExternFn f ret params ->
+  | ExternFn f ret params pure ->
     let ret, ds = translate_typ ret in
     let params, ds = List.fold_left (fun (params, ds) (t, i, _) ->
       let t, ds_t = translate_typ t in
       params@[i, t],ds@ds_t) ([], ds) params in
-    ds @ [with_comments (T.Extern_fn f ret params) (A.is_entrypoint d) false []]
+    ds @ [with_comments (T.Extern_fn f ret params pure) (A.is_entrypoint d) false []]
 
-  | ExternProbe f ->
-    [with_comments (T.Extern_probe f) (A.is_entrypoint d) false []]
+  | ExternProbe f pq ->
+    let translate_qualifier (pq:option A.probe_qualifier) : ML T.probe_qualifier =
+      match pq with
+      | None -> T.PQSimple
+      | Some A.PQWithOffsets -> T.PQWithOffsets
+      | Some (A.PQRead t) -> 
+        T.PQRead t
+      | Some (A.PQWrite t) ->
+        T.PQWrite t
+    in
+    let pq = translate_qualifier pq in
+    [with_comments (T.Extern_probe f pq) (A.is_entrypoint d) false []]
 
 noeq
 type translate_env = {
